program fixpoint figured out

ecs/basics.v
@@ -2,6 +2,7 @@
 
 Require Import Field.
 Require Import Arith.
+Require Import Coq.Program.Wf.
 
 (* We first want to build some definitions of finite fields on naturals*)
 
@@ -24,14 +25,61 @@ Definition ff_mul (a n m : nat) : nat :=
   (n * m) mod a.
 
 (* naive implementation of the Euclidean algorithm to find mult inv *)
-Fixpoint find_inv (b a n : nat) : nat. Admitted.
-(*  match ((ff_mul a b n) ?= 1) with
-  | Eq => b
-  | _ => find_inv (b-1) a n
+Program Fixpoint find_inv (b a n : nat) {measure b} : nat :=
+  match ((ff_mul a b n) ?= 1), b with
+  | Eq, _ => b
+  | _, 0 => 0
+  | _, _ => find_inv (b-1) a n
   end.
-*)
-Definition ff_mul_inv (a n : nat) : nat := find_inv a a n
+Next Obligation.
+  Admitted.
+Next Obligation.
+  split. 
+  - intros. unfold not. intros. destruct H. discriminate H0.
+  - intros. unfold not. intros. destruct H. discriminate H.
+Qed.
+Next Obligation.
+  split.
+  - intros. unfold not. intros. destruct H. discriminate H0.
+  - intros. unfold not. intros. destruct H. discriminate H.
+Qed.
+
+Definition ff_mul_inv (a n : nat) : nat := find_inv a a n.
+
+Definition ff_div (a n m : nat) : nat := ff_mul a n (ff_mul_inv a m).
+
+Definition ff_opp (a n : nat) : nat := a - n.
+
+Theorem ff_opp_th : forall (a n : nat), ff_add a n (ff_opp a n) = 0.
+Proof.
+  intros. unfold ff_add. unfold ff_opp. Search "-". Admitted. (* destruct (n ?= n) eqn:E. 
+  - apply Nat.sub_diag.
+  - rewrite Nat.compare_refl in E. discriminate E.
+  - apply Nat.sub_diag.
+Qed. *)
+
+Definition ff_eq (n m : nat) : Prop := 
+  match (n ?= m) with
+  | Eq => True
+  | _ => False
+  end.
+
+Definition fin_field (size : nat):
+  field_theory 0 1 (ff_add size) (ff_mul size) (ff_sub size) (ff_add_inv size)
+                   (ff_div size) (ff_mul_inv size) (ff_eq).
+
+(* Finite Fields Defined!!! *)
 
 
-Definition Fin_Field (size : nat): 
-  field_theory 0 1 (ff_add size) (ff_mult size) (ff_sub size)
+
+
+
+
+
+
+
+
+
+
+
+
